coq/proof/SoundPostcondForget.v
@@ -29,25 +29,6 @@ Require Import SoundForget.
 Set Implicit Arguments.
 
 
-(* TODO: move this to soundforget.v? *)
-Lemma postcond_cmd_forget_le
-      def_src def_tgt leaks_src leaks_tgt
-      inv:
-  Invariant.le
-    (Forget.t def_src def_tgt leaks_src leaks_tgt inv)
-    inv.
-Proof.
-Admitted.
-
-Lemma postcond_cmd_forget_memory_le
-      def_memory_src def_memory_tgt
-      inv:
-  Invariant.le
-    (ForgetMemory.t def_memory_src def_memory_tgt inv)
-    inv.
-Proof.
-Admitted.
-
 Lemma step_state_equiv_except
       cmd cmds
       conf st0 st1 evt
@@ -66,15 +47,12 @@ Admitted.
 
 Definition FORGET_MEMORY_TODO: Prop. Admitted. (* TODO *)
 
-(* TODO: we can assume source's progress *)
 Lemma postcond_cmd_forget_sound
-      conf_src st0_src st1_src def_src leaks_src cmd_src cmds_src def_memory_src
-      conf_tgt st0_tgt st1_tgt def_tgt leaks_tgt cmd_tgt cmds_tgt def_memory_tgt
+      conf_src st0_src st1_src def_src leaks_src def_memory_src
+      conf_tgt st0_tgt st1_tgt def_tgt leaks_tgt def_memory_tgt
       invst0 invmem0 inv0
       (STATE: InvState.Rel.sem conf_src conf_tgt st0_src st0_tgt invst0 invmem0 inv0)
       (MEM: InvMem.Rel.sem conf_src conf_tgt st0_src.(Mem) st0_tgt.(Mem) invmem0)
-      (CMDS_SRC: st0_src.(EC).(CurCmds) = cmd_src :: cmds_src)
-      (CMDS_TGT: st0_tgt.(EC).(CurCmds) = cmd_tgt :: cmds_tgt)
       (STATE_SRC: state_equiv_except def_src st0_src st1_src)
       (STATE_TGT: state_equiv_except def_tgt st0_tgt st1_tgt)
       (UNIQUE_SRC: unique_preserved_except conf_src invst0.(InvState.Rel.src) inv0.(Invariant.src) st1_src def_src leaks_src)
@@ -85,6 +63,29 @@ Lemma postcond_cmd_forget_sound
     <<STATE: InvState.Rel.sem conf_src conf_tgt st1_src st1_tgt invst1 invmem1
                               (ForgetMemory.t def_memory_src def_memory_tgt
                                               (Forget.t def_src def_tgt leaks_src leaks_tgt inv0)) >> /\
+    <<MEM: InvMem.Rel.sem conf_src conf_tgt st1_src.(Mem) st1_tgt.(Mem) invmem1>> /\
+    <<MEMLE: InvMem.Rel.le invmem0 invmem1>>.
+Proof.
+Admitted.
+
+
+Definition FORGET_MEMORY_CALL_TODO: Prop. Admitted. (* TODO *)
+
+Lemma postcond_call_forget_sound
+      conf_src st0_src st1_src def_src leaks_src
+      conf_tgt st0_tgt st1_tgt def_tgt leaks_tgt
+      invst0 invmem0 inv0
+      (STATE: InvState.Rel.sem conf_src conf_tgt st0_src st0_tgt invst0 invmem0 inv0)
+      (MEM: InvMem.Rel.sem conf_src conf_tgt st0_src.(Mem) st0_tgt.(Mem) invmem0)
+      (STATE_SRC: state_equiv_except def_src st0_src st1_src)
+      (STATE_TGT: state_equiv_except def_tgt st0_tgt st1_tgt)
+      (UNIQUE_SRC: unique_preserved_except conf_src invst0.(InvState.Rel.src) inv0.(Invariant.src) st1_src def_src leaks_src)
+      (UNIQUE_TGT: unique_preserved_except conf_tgt invst0.(InvState.Rel.tgt) inv0.(Invariant.tgt) st1_tgt def_tgt leaks_tgt)
+      (MEM_SRC: FORGET_MEMORY_CALL_TODO)
+      (MEM_TGT: FORGET_MEMORY_CALL_TODO)
+  : exists invst1 invmem1,
+    <<STATE: InvState.Rel.sem conf_src conf_tgt st1_src st1_tgt invst1 invmem1
+                              (ForgetMemoryCall.t (Forget.t def_src def_tgt leaks_src leaks_tgt inv0)) >> /\
     <<MEM: InvMem.Rel.sem conf_src conf_tgt st1_src.(Mem) st1_tgt.(Mem) invmem1>> /\
     <<MEMLE: InvMem.Rel.le invmem0 invmem1>>.
 Proof.
